src/tls/StatefulPlain.fst
@@ -24,9 +24,9 @@ type id = i:id { pv_of_id i <> TLS_1p3 }
 
 let ad_Length i = match pv_of_id i with
     | SSL_3p0 -> 1
-    | _       -> 3 // ContentType[1] + Version[2]
+    | _       -> 3 // contentType[1] + Version[2]
 
-val makeAD: i:id -> ct:ContentType -> Tot (lbytes (ad_Length i))
+val makeAD: i:id -> ct:contentType -> Tot (lbytes (ad_Length i))
 let makeAD i ct =
     let pv   = pv_of_id i in
     let bct  = ctBytes ct in
@@ -39,7 +39,7 @@ let makeAD i ct =
 // that said, we should entirely avoid parsing it.
 type adata (i:id) = b:bytes { exists ct. b = makeAD i ct }
 
-val parseAD: i:id -> ad:adata i -> Tot ContentType
+val parseAD: i:id -> ad:adata i -> Tot contentType
 let parseAD i ad =
     let pv = pv_of_id i in
 //    if pv = TLS_1p3 then 
@@ -53,7 +53,7 @@ let parseAD i ad =
       match parseCT bct, parseVersion bver with
       | Correct ct, Correct ver -> assert (ver = pv); ct
 
-val lemma_makeAD_parseAD: i:id -> ct:ContentType -> Lemma
+val lemma_makeAD_parseAD: i:id -> ct:contentType -> Lemma
   (requires (True))
   (ensures (parseAD i (makeAD i ct) = ct))
   [SMTPat (makeAD i ct)]
