src/tls/TLSConstants.fst
@@ -835,7 +835,7 @@ let rec names_of_cipherSuites css =
                 end
        end
 
-// migrated ContentType to Content.fst (this is internal to TLS)
+// migrated contentType to Content.fst (this is internal to TLS)
 
 val bytes_of_seq: n:nat{ repr_bytes n <= 8 } -> Tot bytes
 let bytes_of_seq sn = bytes_of_int 8 sn
